Fix, simplify and cleanup the tests which use the support flags in EverCrypt (compile_128, compile_vale, etc.)

lib/c/evercrypt_targetconfig.h
@@ -1,27 +1,35 @@
 #ifndef __EVERCRYPT_TARGETCONFIG_H
 #define __EVERCRYPT_TARGETCONFIG_H
 
-/* References:
- * - https://docs.microsoft.com/en-us/cpp/preprocessor/predefined-macros?view=vs-2017
- * - https://sourceforge.net/p/predef/wiki/Architectures/
- */
-
-enum {
-  // TODO: the macros defined in EverCrypt.TargetConfig.h don't extract as
-  // uppercase - fix that
-  target_architecture_name_x86,
-  target_architecture_name_x64,
-  target_architecture_name_arm7,
-  target_architecture_name_arm8,
-  target_architecture_name_systemz,
-  target_architecture_name_powerpc64,
-  target_architecture_name_unknown
-};
-
 #if __has_include("config.h")
 #include "config.h"
 #else
-#define target_architecture target_architecture_name_unknown
+#define TARGET_ARCHITECTURE TARGET_ARCHITECTURE_NAME_UNKNOWN
 #endif
+
+// Those functions are called on non-x64 platforms for which the feature detection
+// is not covered by vale's CPUID support; therefore, we hand-write in C ourselves.
+// For now, on non-x64 platforms, if we can compile 128-bit vector code, we can
+// also execute it; this is true of: Z, Power, ARM8. In the future, if we consider
+// cross-compilation scenarios, we'll have to refine this predicate; it could be the case,
+// for instance, that we want our code to run on old revisions of a system without
+// vector instructions, in which case we'll have to do run-time feature detection
+// in addition to compile-time detection.
+
+static inline bool has_vec128_not_avx () {
+#if (TARGET_ARCHITECTURE != TARGET_ARCHITECTURE_NAME_X64) && COMPILE_128
+  return true;
+#else
+  return false;
+#endif
+}
+
+static inline bool has_vec256_not_avx2 () {
+#if (TARGET_ARCHITECTURE != TARGET_ARCHITECTURE_NAME_X64) && COMPILE_256
+  return true;
+#else
+  return false;
+#endif
+}
 
 #endif
