providers/evercrypt/fst/EverCrypt.AEAD.fst
@@ -128,10 +128,8 @@ fun r dst k ->
   let has_avx = EverCrypt.AutoConfig2.has_avx() in
   let has_sse = EverCrypt.AutoConfig2.has_sse() in
   let has_movbe = EverCrypt.AutoConfig2.has_movbe() in
-  if EverCrypt.TargetConfig.compile_vale then
-  if EverCrypt.TargetConfig.compile_128 &&
-     (EverCrypt.TargetConfig.target_architecture = EverCrypt.TargetConfig.target_architecture_name_x64) then
-  if (has_aesni && has_pclmulqdq && has_avx && has_sse && has_movbe) then (
+  if EverCrypt.TargetConfig.compile_vale &&
+     (has_aesni && has_pclmulqdq && has_avx && has_sse && has_movbe) then (
     let ek = B.malloc r 0uy (concrete_xkey_len i + 176ul) in
 
     vale_expand i k ek;
@@ -147,11 +145,6 @@ fun r dst k ->
 
   ) else
     UnsupportedAlgorithm
-  else
-    UnsupportedAlgorithm
-  else
-    UnsupportedAlgorithm
-
 
 let create_in_aes128_gcm: create_in_st AES128_GCM = create_in_aes_gcm Vale_AES128
 let create_in_aes256_gcm: create_in_st AES256_GCM = create_in_aes_gcm Vale_AES256
@@ -318,38 +311,20 @@ fun s iv iv_len ad ad_len plain plain_len cipher tag ->
       pop_frame();
       Success
 
-let encrypt_aes128_gcm (_: squash (
-      EverCrypt.TargetConfig.compile_vale /\
-      EverCrypt.TargetConfig.compile_128 /\
-      EverCrypt.TargetConfig.target_architecture = EverCrypt.TargetConfig.target_architecture_name_x64)):
+let encrypt_aes128_gcm (_: squash (EverCrypt.TargetConfig.compile_vale)):
   encrypt_st AES128_GCM =
   fun s iv iv_len ad ad_len plain plain_len cipher tag ->
     if EverCrypt.TargetConfig.compile_vale then
-    if EverCrypt.TargetConfig.compile_128 &&
-       (EverCrypt.TargetConfig.target_architecture = EverCrypt.TargetConfig.target_architecture_name_x64)
-    then
       encrypt_aes_gcm Vale_AES128 s iv iv_len ad ad_len plain plain_len cipher tag
     else
       let () = false_elim () in
       LowStar.Failure.failwith "statically unreachable"
-    else
-      let () = false_elim () in
-      LowStar.Failure.failwith "statically unreachable"
 
-let encrypt_aes256_gcm (_: squash (
-      EverCrypt.TargetConfig.compile_vale /\
-      EverCrypt.TargetConfig.compile_128 /\
-      EverCrypt.TargetConfig.target_architecture = EverCrypt.TargetConfig.target_architecture_name_x64)):
+let encrypt_aes256_gcm (_: squash (EverCrypt.TargetConfig.compile_vale)):
   encrypt_st AES256_GCM =
   fun s iv iv_len ad ad_len plain plain_len cipher tag ->
     if EverCrypt.TargetConfig.compile_vale then
-    if EverCrypt.TargetConfig.compile_128 &&
-       (EverCrypt.TargetConfig.target_architecture = EverCrypt.TargetConfig.target_architecture_name_x64)
-    then
       encrypt_aes_gcm Vale_AES256 s iv iv_len ad ad_len plain plain_len cipher tag
-    else
-      let () = false_elim () in
-      LowStar.Failure.failwith "statically unreachable"
     else
       let () = false_elim () in
       LowStar.Failure.failwith "statically unreachable"
@@ -402,15 +377,9 @@ let encrypt_expand_aes128_gcm : encrypt_expand_st true AES128_GCM =
   let has_sse = EverCrypt.AutoConfig2.has_sse() in
   let has_movbe = EverCrypt.AutoConfig2.has_movbe() in
   let has_aesni = EverCrypt.AutoConfig2.has_aesni () in
-  if EverCrypt.TargetConfig.compile_vale then
-  if EverCrypt.TargetConfig.compile_128 &&
-     (EverCrypt.TargetConfig.target_architecture = EverCrypt.TargetConfig.target_architecture_name_x64) then
-  if has_aesni && has_pclmulqdq && has_avx && has_sse && has_movbe then
+  if EverCrypt.TargetConfig.compile_vale &&
+     (has_aesni && has_pclmulqdq && has_avx && has_sse && has_movbe) then
     encrypt_expand_aes_gcm Vale_AES128 k iv iv_len ad ad_len plain plain_len cipher tag
-  else
-    UnsupportedAlgorithm
-  else
-    UnsupportedAlgorithm
   else
     UnsupportedAlgorithm
 
@@ -421,15 +390,9 @@ let encrypt_expand_aes256_gcm : encrypt_expand_st true AES256_GCM =
   let has_sse = EverCrypt.AutoConfig2.has_sse() in
   let has_movbe = EverCrypt.AutoConfig2.has_movbe() in
   let has_aesni = EverCrypt.AutoConfig2.has_aesni () in
-  if EverCrypt.TargetConfig.compile_vale then
-  if EverCrypt.TargetConfig.compile_128 &&
-     (EverCrypt.TargetConfig.target_architecture = EverCrypt.TargetConfig.target_architecture_name_x64) then
-  if has_aesni && has_pclmulqdq && has_avx && has_sse && has_movbe then
+  if EverCrypt.TargetConfig.compile_vale &&
+     (has_aesni && has_pclmulqdq && has_avx && has_sse && has_movbe) then
     encrypt_expand_aes_gcm Vale_AES256 k iv iv_len ad ad_len plain plain_len cipher tag
-  else
-    UnsupportedAlgorithm
-  else
-    UnsupportedAlgorithm
   else
     UnsupportedAlgorithm
 
@@ -574,42 +537,23 @@ fun s iv iv_len ad ad_len cipher cipher_len tag dst ->
         else
           AuthenticationFailure
 
-let decrypt_aes128_gcm (_: squash (
-      EverCrypt.TargetConfig.compile_vale /\
-      EverCrypt.TargetConfig.compile_128 /\
-      EverCrypt.TargetConfig.target_architecture = EverCrypt.TargetConfig.target_architecture_name_x64)):
+let decrypt_aes128_gcm (_: squash (EverCrypt.TargetConfig.compile_vale)):
   decrypt_st AES128_GCM =
   fun s iv iv_len ad ad_len cipher cipher_len tag dst ->
     if EverCrypt.TargetConfig.compile_vale then
-    if EverCrypt.TargetConfig.compile_128 &&
-       (EverCrypt.TargetConfig.target_architecture = EverCrypt.TargetConfig.target_architecture_name_x64)
-    then
       decrypt_aes_gcm Vale_AES128 s iv iv_len ad ad_len cipher cipher_len tag dst
     else
       let () = false_elim () in
       LowStar.Failure.failwith "statically unreachable"
-    else
-      let () = false_elim () in
-      LowStar.Failure.failwith "statically unreachable"
 
-let decrypt_aes256_gcm (_: squash (
-      EverCrypt.TargetConfig.compile_vale /\
-      EverCrypt.TargetConfig.compile_128 /\
-      EverCrypt.TargetConfig.target_architecture = EverCrypt.TargetConfig.target_architecture_name_x64)):
+let decrypt_aes256_gcm (_: squash (EverCrypt.TargetConfig.compile_vale)):
   decrypt_st AES256_GCM =
   fun s iv iv_len ad ad_len cipher cipher_len tag dst ->
     if EverCrypt.TargetConfig.compile_vale then
-    if EverCrypt.TargetConfig.compile_128 &&
-       (EverCrypt.TargetConfig.target_architecture = EverCrypt.TargetConfig.target_architecture_name_x64)
-    then
       decrypt_aes_gcm Vale_AES256 s iv iv_len ad ad_len cipher cipher_len tag dst
     else
       let () = false_elim () in
       LowStar.Failure.failwith "statically unreachable"
-    else
-      let () = false_elim () in
-      LowStar.Failure.failwith "statically unreachable"
-
 
 let decrypt_chacha20_poly1305 : decrypt_st CHACHA20_POLY1305 =
   fun s iv iv_len ad ad_len cipher cipher_len tag dst ->
@@ -681,15 +625,9 @@ let decrypt_expand_aes128_gcm : decrypt_expand_st true AES128_GCM =
   let has_sse = EverCrypt.AutoConfig2.has_sse() in
   let has_movbe = EverCrypt.AutoConfig2.has_movbe() in
   let has_aesni = EverCrypt.AutoConfig2.has_aesni () in
-  if EverCrypt.TargetConfig.compile_vale then
-  if EverCrypt.TargetConfig.compile_128 &&
-     (EverCrypt.TargetConfig.target_architecture = EverCrypt.TargetConfig.target_architecture_name_x64) then
-  if has_aesni && has_pclmulqdq && has_avx && has_sse && has_movbe then
+  if EverCrypt.TargetConfig.compile_vale &&
+     (has_aesni && has_pclmulqdq && has_avx && has_sse && has_movbe) then
     decrypt_expand_aes_gcm Vale_AES128 k iv iv_len ad ad_len cipher cipher_len tag dst
-  else
-    UnsupportedAlgorithm
-  else
-    UnsupportedAlgorithm
   else
     UnsupportedAlgorithm
 
@@ -700,15 +638,9 @@ let decrypt_expand_aes256_gcm : decrypt_expand_st true AES256_GCM =
   let has_sse = EverCrypt.AutoConfig2.has_sse() in
   let has_movbe = EverCrypt.AutoConfig2.has_movbe() in
   let has_aesni = EverCrypt.AutoConfig2.has_aesni () in
-  if EverCrypt.TargetConfig.compile_vale then
-  if EverCrypt.TargetConfig.compile_128 &&
-     (EverCrypt.TargetConfig.target_architecture = EverCrypt.TargetConfig.target_architecture_name_x64) then
-  if has_aesni && has_pclmulqdq && has_avx && has_sse && has_movbe then
+  if EverCrypt.TargetConfig.compile_vale &&
+     (has_aesni && has_pclmulqdq && has_avx && has_sse && has_movbe) then
     decrypt_expand_aes_gcm Vale_AES256 k iv iv_len ad ad_len cipher cipher_len tag dst
-  else
-    UnsupportedAlgorithm
-  else
-    UnsupportedAlgorithm
   else
     UnsupportedAlgorithm
 
