providers/evercrypt/fst/EverCrypt.CTR.fst
@@ -46,8 +46,6 @@ let cpu_features_invariant (i: impl): Type0 =
   match i with
   | Vale_AES128 | Vale_AES256 ->
       EverCrypt.TargetConfig.compile_vale /\
-      EverCrypt.TargetConfig.compile_128 /\
-      EverCrypt.TargetConfig.target_architecture = EverCrypt.TargetConfig.target_architecture_name_x64 /\
       Vale.X64.CPU_Features_s.(aesni_enabled /\ pclmulqdq_enabled /\ avx_enabled /\ sse_enabled)
   | Hacl_CHACHA20 ->
       True
@@ -113,12 +111,7 @@ fun r dst k iv iv_len c ->
   if iv_len `UInt32.lt` 12ul then
     InvalidIVLength
 
-  else if EverCrypt.TargetConfig.compile_vale then
-  // This is a bit annoying: EverCrypt.TargetConfig.compile_128 won't be
-  // translated as an if-def if we group the two below ifs
-  if EverCrypt.TargetConfig.compile_128 then
-  if EverCrypt.TargetConfig.target_architecture = EverCrypt.TargetConfig.target_architecture_name_x64 &&
-     has_aesni && has_pclmulqdq && has_avx && has_sse then
+  else if EverCrypt.TargetConfig.compile_vale && (has_aesni && has_pclmulqdq && has_avx && has_sse) then
     (**) let h0 = ST.get () in
     (**) let g_iv = G.hide (B.as_seq h0 iv) in
     (**) let g_key: G.erased (key a) = G.hide (B.as_seq h0 (k <: B.buffer uint8)) in
@@ -143,12 +136,6 @@ fun r dst k iv iv_len c ->
     (**) B.modifies_only_not_unused_in B.(loc_buffer dst) h0 h4;
 
     Success
-
-  else
-    UnsupportedAlgorithm
-
-  else
-    UnsupportedAlgorithm
 
   else
     UnsupportedAlgorithm
@@ -203,13 +190,9 @@ let copy_or_expand (i: impl)
   match i with
   | Vale_AES128 ->
     if EverCrypt.TargetConfig.compile_vale then
-    if EverCrypt.TargetConfig.compile_128 then
-    if EverCrypt.TargetConfig.target_architecture = EverCrypt.TargetConfig.target_architecture_name_x64 then
         vale_expand Vale_AES128 k ek
   | Vale_AES256 ->
     if EverCrypt.TargetConfig.compile_vale then
-    if EverCrypt.TargetConfig.compile_128 then
-    if EverCrypt.TargetConfig.target_architecture = EverCrypt.TargetConfig.target_architecture_name_x64 then
         vale_expand Vale_AES256 k ek
   | Hacl_CHACHA20 ->
       B.blit k 0ul ek 0ul 32ul
@@ -354,14 +337,10 @@ let update_block a p dst src =
   match i with
   | Vale_AES128 ->
     if EverCrypt.TargetConfig.compile_vale then
-    if EverCrypt.TargetConfig.compile_128 then
-    if EverCrypt.TargetConfig.target_architecture = EverCrypt.TargetConfig.target_architecture_name_x64 then
         update_block_vale Vale_AES128 p dst src
 
   | Vale_AES256 ->
     if EverCrypt.TargetConfig.compile_vale then
-    if EverCrypt.TargetConfig.compile_128 then
-    if EverCrypt.TargetConfig.target_architecture = EverCrypt.TargetConfig.target_architecture_name_x64 then
         update_block_vale Vale_AES256 p dst src
 
   | Hacl_CHACHA20 ->
